src/Reflection/MapCast.v
@@ -34,10 +34,17 @@ Section language.
     Context {ovar : base_type_code1 -> Type}.
     Local Notation ivar t := (@exprf base_type_code1 op1 ovar (Tbase t)) (only parsing).
     Local Notation ivarf := (fun t => ivar t).
-    Context (transfer_var : forall tx1 tx2 tC1
-                                   (f : interp_flat_type ivarf tx1 -> exprf base_type_code1 op1 (var:=ovar) tC1)
-                                   (v : interp_flat_type ivarf tx2),
-                exprf base_type_code1 op1 (var:=ovar) tC1).
+    Context (transfer_var1 : forall tx1 tx2
+                                    (v1 : ivar tx1)
+                                    (v2 : interp_base_type2 tx2),
+                exprf base_type_code1 op1 (var:=ovar) (Tbase (new_base_type tx2 v2))).
+    Context (transfer_var2 : forall tx1
+                                    tx' tC'
+                                    (ex' : interp_flat_type interp_base_type2 tx')
+                                    (eC' : interp_flat_type interp_base_type2 tx' -> exprf base_type_code2 op2 tC')
+                                    (f : interp_flat_type ivarf tx1 -> exprf base_type_code1 op1 (var:=ovar) (new_flat_type (interpf interp_op2 (eC' ex'))))
+                                    (v : interp_flat_type ovar (new_flat_type ex')),
+                exprf base_type_code1 op1 (var:=ovar) (new_flat_type (interpf interp_op2 (eC' ex')))).
     Local Notation SmartFail
       := (SmartValf _ (@failv _)).
     Local Notation failf t (* {t} : @exprf base_type_code1 op1 ovar t*)
@@ -55,8 +62,8 @@ Section language.
       := match e1 in exprf _ _ t1, e2 as e2 in exprf _ _ t2
                return exprf _ _ (var:=ovar) (@new_flat_type _ (interpf interp_op2 e2)) with
          | TT, TT => TT
-         | Var tx1 x1, Var tx2 x2 as e2'
-           => transfer_var (Tbase _) (Tbase _) (Tbase _) (fun x => x) x1
+         | Var tx1 x1, Var tx2 x2
+           => transfer_var1 _ _ x1 x2
          | Op _ tR1 op1 args1, Op _ tR2 op2 args2
            => let args' := @mapf_interp_cast _ args1 _ args2 in
               transfer_op _ _ _ _ _ op1 op2 args2 args'
@@ -64,7 +71,7 @@ Section language.
            => let ex' := @mapf_interp_cast _ ex1 _ ex2 in
               let eC' := fun v' => @mapf_interp_cast _ (eC1 v') _ (eC2 (interpf interp_op2 ex2)) in
               LetIn ex'
-                    (fun v => transfer_var _ _ _ eC' (SmartVarfMap (fun t => Var) v))
+                    (fun v => transfer_var2 _ _ _ (interpf interp_op2 ex2) eC2 eC' v)
          | Pair tx1 ex1 ty1 ey1, Pair tx2 ex2 ty2 ey2
            => Pair
                 (@mapf_interp_cast _ ex1 _ ex2)
@@ -78,23 +85,24 @@ Section language.
          end.
     Arguments mapf_interp_cast {_} _ {_} _. (* 8.4 workaround for bad arguments *)
 
+
     Definition map_interp_cast
              {t1} (e1 : @expr base_type_code1 op1 ivarf t1)
              {t2} (e2 : @expr base_type_code2 op2 interp_base_type2 t2)
-      : forall (args2 : interp_flat_type interp_base_type2 (domain t2)),
-        @expr base_type_code1 op1 ovar (@new_type _ args2 (interp interp_op2 e2))
-      := match e1 in expr _ _ t1, e2 in expr _ _ t2
-               return forall (args2 : interp_flat_type _ (domain t2)), expr _ _ (new_type _ args2 (interp _ e2)) with
-         | Abs src1 dst1 f1, Abs src2 dst2 f2
-           => fun args2
-              => Abs (fun x : interp_flat_type _ (new_flat_type _)
-                      => transfer_var _ _ _ (fun x => @mapf_interp_cast _ (f1 x) _ (f2 args2)) (SmartVarfMap (fun t => Var) x))
-         end.
+             (args2 : interp_flat_type interp_base_type2 (domain t2))
+      : @expr base_type_code1 op1 ovar (@new_type _ args2 (interp interp_op2 e2))
+      := let f1 := invert_Abs e1 in
+         let f2 := invert_Abs e2 in
+         Abs (fun x
+              => transfer_var2
+                    _ (domain t2) (codomain t2) args2 (invert_Abs e2)
+                    (fun x => @mapf_interp_cast _ (f1 x) _ (f2 args2))
+                    x).
   End with_var.
 End language.
 
-Global Arguments mapf_interp_cast {_ _ _ _ _ _} failv {_} transfer_op {ovar} transfer_var {t1} e1 {t2} e2.
-Global Arguments map_interp_cast {_ _ _ _ _ _} failv {_} transfer_op {ovar} transfer_var {t1} e1 {t2} e2 args2.
+Global Arguments mapf_interp_cast {_ _ _ _ _ _} failv {_} transfer_op {ovar} transfer_var1 transfer_var2 {t1} e1 {t2} e2.
+Global Arguments map_interp_cast {_ _ _ _ _ _} failv {_} transfer_op {ovar} transfer_var1 transfer_var2 {t1} e1 {t2} e2 args2.
 Global Arguments new_type {_ _ _} new_base_type {t} _ _.
 
 Section homogenous.
@@ -106,13 +114,20 @@ Section homogenous.
           (new_base_type : forall t, interp_base_type2 t -> base_type_code).
 
   Definition MapInterpCast
-          transfer_op
-          (transfer_var : forall ovar tx1 tx2 tC1
-                                 (ivarf := fun t => @exprf base_type_code op ovar (Tbase t))
-                                 (f : interp_flat_type ivarf tx1 -> exprf base_type_code op (var:=ovar) tC1)
-                                 (v : interp_flat_type ivarf tx2),
-              exprf base_type_code op (var:=ovar) tC1)
+             transfer_op
+             (transfer_var1 : forall ovar tx1 tx2
+                                     (v1 : @exprf base_type_code op ovar (Tbase tx1))
+                                     (v2 : interp_base_type2 tx2),
+                 exprf base_type_code op (var:=ovar) (Tbase (new_base_type tx2 v2)))
+             (transfer_var2 : forall ovar tx1
+                                     tx' tC'
+                                     (ivarf := fun t => @exprf base_type_code op ovar (Tbase t))
+                                     (ex' : interp_flat_type interp_base_type2 tx')
+                                     (eC' : interp_flat_type interp_base_type2 tx' -> exprf base_type_code op tC')
+                                     (f : interp_flat_type ivarf tx1 -> exprf base_type_code op (var:=ovar) (_ (interpf interp_op2 (eC' ex'))))
+                                    (v : interp_flat_type ovar (_ ex')),
+                exprf base_type_code op (var:=ovar) (_ (interpf interp_op2 (eC' ex'))))
           {t} (e : Expr base_type_code op t) (args : interp_flat_type interp_base_type2 (domain t))
     : Expr base_type_code op (new_type (@new_base_type) args (Interp interp_op2 e))
-    := fun var => map_interp_cast (@failv) transfer_op (transfer_var _) (e _) (e _) args.
+    := fun var => map_interp_cast (@failv) transfer_op (transfer_var1 _) (transfer_var2 _) (e _) (e _) args.
 End homogenous.
